Commit before extension to SoL

src/tactic/nccc/correct.lean
@@ -1,15 +1,13 @@
-import .search .logic tactic.mono_con
+import .search .logic tactic.monotonicity tactic.fin_cases
 
 variable {α : Type}
 
-local notation `⅋` k   := term.fnc k
-local notation t `&` s := term.tpp t s
-local notation t `#` k := term.vpp t k
+local notation `⅋` k   := atom.fnc k
+local notation a `&` b := atom.app a b
+local notation a `#` k := atom.vpp a k
 
 def goal : Type := cla × cla × mat
 def ext_goal : Type := cla × cla × mat × mat
-
-namespace goal
 
 def is_ext (m x : mat) : Prop :=
 ∀ c ∈ x, ∃ d ∈ m, ∃ σ : sub, c = cla.subst σ d
@@ -55,9 +53,8 @@ begin
   cases h,
 end
 
-lemma rot_path_correct (p c : cla) (m : mat) (k : nat) :
-  ext_valid α (p.rotate k, c, m) →
-  ext_valid α (p, c, m) :=
+lemma rot_path_correct {p c : cla} {m : mat} (k : nat) :
+  ext_valid α (p.rotate k, c, m) → ext_valid α (p, c, m) :=
 begin
   intro h1,
   rcases h1 with ⟨x, h1, h2⟩,
@@ -69,7 +66,60 @@ begin
   right, exact h3,
 end
 
-lemma rot_mat_correct (p c : cla) (m : mat) (k : nat) :
+lemma rot_mat_correct' {m : mat} (k : nat) :
+  mat.fam_exv α (m.rotate k) → mat.fam_exv α m :=
+begin
+  intros h0 M,
+  rcases h0 M with ⟨v, c, h1, h2⟩,
+  refine ⟨v, c, mem_rotate.elim_left h1, h2⟩
+end
+
+lemma exists_ext {c : cla} {m : mat} {k : nat} :
+  ∀ x : mat, is_ext (c.rotate k :: m) x →
+  ∃ y : mat, (is_ext (c :: m) y ∧
+    ∀ M : model α, ∀ v : nat → α, x.holds M v ↔ y.holds M v)
+| []     h0 := ⟨[], forall_mem_nil _, λ M v, iff.refl _⟩
+| (d::x) h0 :=
+  begin
+    rcases exists_ext x (forall_mem_of_forall_mem_cons h0) with ⟨y, h1, h2⟩,
+    rcases h0 d (or.inl rfl) with ⟨e, he1, σ, he2⟩,
+    rw mem_cons_iff at he1, cases he1,
+    { refine ⟨c.subst σ :: y,
+        forall_mem_cons.elim_right
+        ⟨⟨_, or.inl rfl, _, rfl⟩, h1⟩, λ M v, _⟩,
+      have h3 : cla.holds M v d ↔ cla.holds M v (cla.subst σ c),
+      { apply forall_mem_iff_forall_mem_of_seteq,
+        rw [he2, he1],
+        apply map_seteq_map_of_seteq (rotate_seteq_self _ _) },
+      simp only [mat.holds_cons, h2 M v, h3] },
+    refine ⟨d :: y, forall_mem_cons.elim_right
+      ⟨⟨e, or.inr he1, _, he2⟩, h1⟩, λ M v, _⟩,
+    simp only [mat.holds_cons, h2 M v]
+  end
+
+lemma rot_cla_correct {p c d : cla} {m : mat} (k : nat) :
+  ext_valid α (p, c, d.rotate k :: m) →
+  ext_valid α (p, c, d :: m) :=
+begin
+  intro h1,
+  rcases h1 with ⟨x, h1, h2⟩,
+  rcases exists_ext x h1 with ⟨y, h3, h4⟩,
+  refine ⟨y, h3, λ M v, _⟩,
+  rcases h2 M v with h5 | h5 | h5 | h5,
+  { left, exact h5 },
+  { right, left, exact h5 },
+  { right, right, left,
+    rw exists_mem_cons_iff at h5,
+    cases h5,
+    { refine ⟨d, or.inl rfl, _⟩,
+      apply forall_mem_of_subset_of_forall_mem
+        (λ x, mem_rotate.elim_right) h5 },
+    apply exists_mem_cons_of_exists h5 },
+  right, right, right,
+  exact (h4 M v).elim_left h5
+end
+
+lemma rot_mat_correct {p c : cla} {m : mat} (k : nat) :
   ext_valid α (p, c, m.rotate k) →
   ext_valid α (p, c, m) :=
 begin
@@ -90,8 +140,8 @@ begin
   exact h3,
 end
 
-lemma start_copy_correct (c : cla) (m : mat) (σ : sub) :
-  ext_valid α ([], c.subst σ, c :: m) → mat.valsat α (c :: m) :=
+lemma start_copy_correct {c : cla} {m : mat} (σ : sub) :
+  ext_valid α ([], c.subst σ, c :: m) → mat.fam_exv α (c :: m) :=
 begin
   intros h2 M,
   rcases h2 with ⟨x, h2, h3⟩,
@@ -105,8 +155,8 @@ begin
   apply mat.exv_of_holds_ext h2 h4,
 end
 
-lemma start_correct (c : cla) (m : mat) :
-  ext_valid α ([], c, m) → mat.valsat α (c :: m) :=
+lemma start_correct {c : cla} {m : mat} :
+  ext_valid α ([], c, m) → mat.fam_exv α (c :: m) :=
 begin
   intros h1 M,
   rcases h1 with ⟨x, h1, h2⟩,
@@ -120,7 +170,7 @@ begin
   refine ⟨v, exists_mem_cons_of_exists h4⟩,
 end
 
-lemma red_correct (l n : lit) (p c : cla) (m : mat) :
+lemma red_correct {l n : lit} {p c : cla} {m : mat} :
   l.neg = n → ext_valid α (n :: p, c, m) → ext_valid α (n :: p, l :: c, m) :=
 begin
   intros h1 h2,
@@ -141,7 +191,7 @@ begin
   exact h4,
 end
 
-lemma ext_copy_correct (l n : lit) (p c d : cla) (m : mat) (σ : sub) :
+lemma ext_copy_correct {l n : lit} {p c d : cla} {m : mat} (σ : sub) :
   l.neg = n.subst σ →
   ext_valid α (p, c, (n :: d) :: m) →
   ext_valid α (l :: p, d.subst σ, (n :: d) :: m) →
@@ -192,7 +242,7 @@ begin
   left, exact h6
 end
 
-lemma ext_correct (l n : lit) (p c d : cla) (m : mat) :
+lemma ext_correct {l n : lit} {p c d : cla} {m : mat} :
   l.neg = n →
   ext_valid α (p, c, (n :: d) :: m) →
   ext_valid α (l :: p, d, m) →
@@ -238,330 +288,3 @@ begin
   rw exists_mem_append_iff,
   left, exact h6
 end
-
-
-#exit
-
-
-
-
-
-lemma start_some_correct (m : mat) (j : nat) (h1 : j < m.length) (σ : sub) :
-  ext_valid α ([], (m.nth_le j h1).subst σ, m) → m.valsat α :=
-begin
-  intros h2 M,
-  rcases h2 with ⟨x, h2, h3⟩,
-  cases h3 M (λ _, M.inhab) with h4 h4,
-  { rcases h4 with ⟨_, h4, _⟩, cases h4 },
-  cases h4,
-  { refine ⟨val.subst M (λ _, M.inhab) σ,
-    m.nth_le j h1, nth_le_mem _ _ _, _⟩,
-    rw [←cla.holds_subst], exact h4 },
-  cases h4,
-  { rcases h4 with ⟨d, h5, h6⟩,
-    refine ⟨(λ _, M.inhab), _, h5, h6⟩ },
-  apply mat.exv_of_holds_ext h2 h4,
-end
-lemma start_none_correct (m : mat) (j : nat) (h1 : j < m.length) :
-  ext_valid α ([], m.nth_le j h1, m.except j) → m.valsat α :=
-begin
-  intros h2 M,
-  rcases h2 with ⟨x, h2, h3⟩,
-  cases h3 M (λ _, M.inhab) with h4 h4,
-  { rcases h4 with ⟨_, h4, _⟩, cases h4 },
-  cases h4,
-  refine ⟨(λ _, M.inhab), _, nth_le_mem _ _ _, h4⟩,
-  cases h4,
-  { rcases h4 with ⟨d, h5, h6⟩,
-    refine ⟨(λ _, M.inhab), _, except_subset_self h5, h6⟩ },
-  apply mat.exv_of_holds_ext
-    (is_ext_of_subset_of_is_ext except_subset_self h2) h4,
-end
-
-
-lemma red_correct (l : lit) (c : cla) (m : mat) (p : cla) :
-  l.neg ∈ p → ext_valid α (p, c, m) → ext_valid α (p, l :: c, m) :=
-begin
-  intro h1,
-  rintro ⟨x, h2, h3⟩,
-  refine ⟨x, h2, _⟩,
-  intros M v,
-  cases (h3 M v) with h4 h4,
-  { left, exact h4 },
-  cases h4,
-  { cases classical.em (l.holds M v) with h5 h5,
-    { right, left, rw forall_mem_cons,
-      constructor; assumption },
-    { left, refine ⟨l.neg, h1, _⟩,
-      rw lit.holds_neg, exact h5 } },
-  right, right, exact h4 ,
-end
-
-lemma ext_some_correct (p : cla) (l : lit) (c : cla) (m : mat) (σ : sub)
-  (i j : nat) (h1 : j < m.length) (h2 : i < (m.nth_le j h1).length) :
-  let d := (m.nth_le j h1).subst σ in
-  let n := d.nth_le i (by simpa only [d, cla.subst, length_map] using h2) in
-  l.neg = n →
-  ext_valid α (p, c, m) →
-  ext_valid α (l :: p, d.except i, m) →
-  ext_valid α (p, l :: c, m) :=
-begin
-  intros d n h3 h4 h5,
-  rcases h4 with ⟨x, h4, h6⟩,
-  rcases h5 with ⟨y, h5, h7⟩,
-  refine ⟨d :: (x ++ y), λ e he, _, _⟩,
-  { rw mem_cons_iff at he,
-    cases he,
-    { refine ⟨nth_le m j h1, nth_le_mem _ _ _, σ, _⟩,
-      rw he },
-    rw mem_append at he,
-    cases he,
-    exact (h4 e he),
-    exact (h5 e he) },
-  intros M v,
-  cases (h6 M v) with h6 h6,
-  { left, exact h6 },
-  cases h6 with h6 h6,
-  { cases classical.em (l.holds M v) with hl hl,
-    { right, left, rw forall_mem_cons,
-      constructor; assumption },
-    cases (h7 M v) with h7 h7,
-    { rcases h7 with ⟨k, hk1, hk2⟩,
-      cases hk1,
-      { subst hk1, exfalso, exact hl hk2 },
-      left, refine ⟨k, hk1, hk2⟩ },
-    cases h7 with h7 h7,
-    { right, right, right,
-      refine ⟨d, or.inl rfl, _⟩,  }
-
-
-
-   }
-
-
-end
-
-
-#exit
-
-| ext' {M : mat} {C P : cla} {L : lit} {σ : sub} {i j : nat}
-  {h1 : j < M.length} {h2 : i < (M.nth_le j h1).length} :
-  let D := (M.nth_le j h1).subst σ in
-  let N := ((M.nth_le j h1).nth_le i h2).subst σ in
-  proof C M P →
-  N = L.neg →
-  proof (D.except i) M (L::P) →
-  proof (L::C) M P
-lemma ext_none_correct (l : lit) (c : cla) (m : mat) (p : cla)
-  (i j : nat) (h1 : j < m.length) (h2 : i < (m.nth_le j h1).length) :
-  l.neg = (m.nth_le j h1).nth_le i h2 →
-  ext_valid α (p, c, m) →
-  ext_valid α (l :: p, (m.nth_le j h1).except i, m.except j) →
-  ext_valid α (p, l :: c, m) :=
-begin
-  intros h3 h4 h5,
-  rcases h4 with ⟨x, h4, h6⟩,
-  rcases h5 with ⟨y, h5, h7⟩,
-  refine ⟨x ++ y, ⟨λ d hd, _, _⟩⟩,
-  { rw mem_append at hd,
-    cases hd,
-    exact (h4 d hd),
-    rcases (h5 d hd) with ⟨e, h8, h9⟩,
-    refine ⟨e, except_subset_self h8, h9⟩ },
-  intros M v,
-
-end
-
-#exit
-
-| ext {M : mat} {C P : cla} {L : lit} (i j : nat)
-  {h1 : j < M.length} {h2 : i < (M.nth_le j h1).length} :
-  let D := M.nth_le j h1 in
-  let N := D.nth_le i h2 in
-  proof C M P →
-  N = L.neg →
-  proof (D.except i) (M.except j) (L::P) →
-  proof (L::C) M P
-
-
-def holds (M : model α) (v : nat → α) : goal → Prop
-| (c, m, p) := (cla.holds M v c ∨ ∃ d ∈ m, cla.holds M v d) ∧ (∀ l ∈ p, ¬ lit.holds M v l)
-
-def valsat (α : Type) (g : goal) : Prop :=
-∀ M : model α, ∃ v : nat → α, (holds M v g)
-
-end goal
-
-open list
-
-#check tactic.interactive.rcades
-lemma start_none_correct (m : mat) (j : nat) (h1 : j < m.length) :
-  goal.valsat α (m.nth_le j h1, m.except j, []) → m.valsat α :=
-begin
-  intros h2 M,
-  rcases (h2 M) with ⟨v, h3, h4⟩,
-  refine ⟨v, _⟩, cases h3,
-  { refine ⟨_, nth_le_mem _ _ _, h3⟩ },
-  { rcases h3 with ⟨c, h5, h6⟩,
-    refine ⟨c, mem_of_mem_except h5, h6⟩ }
-end
-
-lemma start_some_correct (m : mat) (j : nat) (h1 : j < m.length) (σ : sub) :
-  goal.valsat α ((m.nth_le j h1).subst σ, m, []) → m.valsat α :=
-begin
-  intros h2 M,
-  rcases (h2 M) with ⟨v, h3, h4⟩,
-  cases h3,
-  refine ⟨val.subst M v σ, m.nth_le j h1,
-    nth_le_mem _ _ _, cla.holds_subst.elim_left h3⟩,
-  refine ⟨v, h3⟩,
-end
-
-lemma red_correct (l : lit) (c : cla) (m : mat) (p : cla) :
-  l.neg ∈ p → goal.valsat α (c, m, p) → goal.valsat α (l :: c, m, p) :=
-begin
-  intros h1 h2 M,
-  rcases h2 M with ⟨v, h3, h4⟩,
-  refine ⟨v, _, h4⟩,
-  cases h3 with h5 h6,
-  { left,
-    apply list.forall_mem_cons.elim_right ⟨ _, h5⟩,
-    apply classical.not_not.elim_left,
-    rw ← lit.holds_neg,
-    exact h4 _ h1 },
-  { right, exact h6 }
-end
-
-
-
-#exit
-
-
-inductive rule : Type
-| start : nat → option sub → rule
-| red   : rule
-| ext   : nat → nat → option sub → rule
-
-def goal : Type := option cla × mat × cla
-
-open rule
-
-def check : list rule → list goal → bool
-| (r :: rs) ((some [], _, _) :: gs) := check rs gs
-| (start j none :: rs) [(none, M, [])] :=
-  if h : j < M.length
-  then check rs [((M.nth_le j h), (M.except j), [])]
-  else ff
-| (start j (some σ) :: rs) [(none, M, [])] :=
-  if h : j < M.length
-  then check rs [((M.nth_le j h).subst σ, M, [])]
-  else ff
-| (red :: rs) ((some (L :: C), M, P) :: gs) :=
-  if L.neg ∈ P
-  then check rs ((some C, M, P) :: gs)
-  else ff
-| (ext j i none :: rs) ((some (L :: C), M, P) :: gs) :=
-  if h1 : j < M.length
-  then if h2 : i < (M.nth_le j h1).length
-       then let D := M.nth_le j h1 in
-            let N := D.nth_le i h2 in
-            (N = L.neg) &&
-              check rs ((C, M, P) :: (D.except i, M.except j, L :: P) :: gs)
-       else ff
-  else ff
-| (ext j i (some σ) :: rs) ((some (L :: C), M, P) :: gs) :=
-  if h1 : j < M.length
-  then if h2 : i < (M.nth_le j h1).length
-       then let D := M.nth_le j h1 in
-            let Dσ := D.subst σ in
-            let Nσ := (D.nth_le i h2).subst σ  in
-            (Nσ = L.neg) &&
-              check rs ((C, M, P) :: (D.except i, M, L :: P) :: gs)
-       else ff
-  else ff
-
-#print axioms check
-
-
-#exit
-
-
-| (rule.start j (some σx) :: rs) none M [] :=
-  do ⟨_, h⟩ ← get_lt_proof j M.length,
-     σ ← σx.inst,
-     (rs', π) ← of_rules rs ((M.nth_le j h).subst σ) M [],
-     return (rs', proof.start' π)
-
-
-#exit
-inductive proof : option cla → mat → cla → Type
-| start {M : mat} {j : nat} {h : j < M.length} :
-  proof (M.nth_le j h) (M.except j) [] →
-  proof none M []
-| start' {M : mat} {j : nat} {h : j < M.length} {σ : sub} :
-  proof ((M.nth_le j h).subst σ) M [] →
-  proof none M []
-| red {M : mat} {C P : cla} {L : lit} :
-  L.neg ∈ P → proof C M P → proof (L::C) M P
-| ext {M : mat} {C P : cla} {L : lit} (i j : nat)
-  {h1 : j < M.length} {h2 : i < (M.nth_le j h1).length} :
-  let D := M.nth_le j h1 in
-  let N := D.nth_le i h2 in
-  proof C M P →
-  N = L.neg →
-  proof (D.except i) (M.except j) (L::P) →
-  proof (L::C) M P
-| ext' {M : mat} {C P : cla} {L : lit} {σ : sub} {i j : nat}
-  {h1 : j < M.length} {h2 : i < (M.nth_le j h1).length} :
-  let D := (M.nth_le j h1).subst σ in
-  let N := ((M.nth_le j h1).nth_le i h2).subst σ in
-  proof C M P →
-  N = L.neg →
-  proof (D.except i) M (L::P) →
-  proof (L::C) M P
-| axm {M : mat} {P : cla} : proof (some []) M P
-
-open tactic
-
-meta def get_lt_proof (m n : nat) : tactic (@subtype unit (λ _, m < n)) :=
-if h : m < n then return (subtype.mk () h) else failed
-
-meta def get_proof (P : Prop) [decidable P] : tactic (@subtype unit (λ _, P)) :=
-if h : P then return (subtype.mk () h) else failed
-
-meta def subx.inst_aux (ktx : nat × expr) : tactic (nat × term) :=
-do t ← eval_expr term ktx.snd, return (ktx.fst, t)
-
-meta def subx.inst (σx : subx) : tactic sub :=
-monad.mapm subx.inst_aux σx
-
-meta def of_rules : list rule → ∀ C : option cla,
-  ∀ M : mat, ∀ P : cla, tactic (list rule × proof C M P)
-| (rule.start j none :: rs) none M [] :=
-  do ⟨_, h⟩ ← get_lt_proof j M.length,
-     (rs', π) ← of_rules rs (M.nth_le j h) (M.except j) [],
-     return (rs', proof.start π)
-| (rule.start j (some σx) :: rs) none M [] :=
-  do ⟨_, h⟩ ← get_lt_proof j M.length,
-     σ ← σx.inst,
-     (rs', π) ← of_rules rs ((M.nth_le j h).subst σ) M [],
-     return (rs', proof.start' π)
-| (rule.red :: rs) (some (L::C)) M P :=
-  do ⟨_, h⟩ ← get_proof (L.neg ∈ P),
-     (rs', π) ← of_rules rs (some C) M P,
-     return (rs', proof.red h π)
-
-
-
-#exit
-  if h : j < M.length
-  then do (rs', π) ← of_rules rs (M.nth_le j h) (M.except j) [],
-          return (rs', proof.start π)
-  else failed
-
-#exit
---lemma valsat_goal_of_proof {α : Type} (M : mat)  :
---  proof none M [] → M.valsat α := sorry
-
-lemma valsat_of_proof {α : Type} (M : mat) :
-  proof none M [] → M.valsat α := sorry
