src/tactic/nccc/mat.lean
@@ -1,4 +1,4 @@
-import .form
+import .form .list
 
 variable {α : Type}
 
@@ -14,7 +14,7 @@ local notation  `∃*` := form.ex
 
 namespace cla
 
-def is_pos (C : cla) : bool := C.all lit.sign
+def is_pos (C : cla) : bool := C.all prod.fst
 
 def vdxs (C : cla) : list nat := ⋃ (C.map lit.vdxs)
 
@@ -22,24 +22,22 @@ def holds (M : model α) (v : nat → α) (c : cla) : Prop :=
 ∀ l ∈ c, lit.holds M v l
 
 def subst : sub → cla → cla :=
-list.map ∘ lit.subst 
+list.map ∘ lit.subst
 
 lemma holds_subst {M : model α} {v : nat → α} {σ : sub} {c : cla} :
-  holds M v (c.subst σ) ↔ holds M (val.subst M v σ) c :=  
+  holds M v (c.subst σ) ↔ holds M (val.subst M v σ) c :=
 begin
   constructor; intros h1 l h2,
-  { rw ← lit.holds_subst, apply h1, 
+  { rw ← lit.holds_subst, apply h1,
     apply list.mem_map_of_mem _ h2 },
   { have h3 : ∃ x, x ∈ c ∧ lit.subst σ x = l,
     { rw ← list.mem_map, exact h2 },
-    rcases h3 with ⟨x, h3, h4⟩, 
+    rcases h3 with ⟨x, h3, h4⟩,
     rw [←h4, lit.holds_subst],
-    apply h1 _ h3 } 
+    apply h1 _ h3 }
 end
-  
+
 end cla
-
-
 
 @[reducible] def mat : Type := list cla
 
@@ -48,7 +46,11 @@ namespace mat
 def holds (M : model α) (v : nat → α) (A : mat) : Prop :=
 ∃ C ∈ A, cla.holds M v C
 
-def valsat (α m) : Prop :=
+lemma holds_cons {M : model α} {v : nat → α} (c : cla) (m : mat) :
+mat.holds M v (c :: m) ↔ (c.holds M v ∨ m.holds M v) :=
+by simp only [mat.holds, list.exists_mem_cons_iff]
+
+def fam_exv (α m) : Prop :=
 ∀ M : model α, ∃ v : nat → α, (holds M v m)
 
 end mat
@@ -62,11 +64,34 @@ def dnf : form → mat
 | (∀* p)   := [] -- Irrelevant
 | (∃* p)   := [] -- Irrelevant
 
-lemma form_valsat_of_mat_valsat (α : Type) (p : form) :
-  p.quant_free → (dnf p).valsat α → p.valsat α := sorry
+open list
 
+lemma holds_of_dnf_holds {M : model α} {v : nat → α} :
+  ∀ p : form, quant_free p → (dnf p).holds M v → p.holds M v :=
+begin
+  form.induce; intros h1 h2;
+  rcases h2 with ⟨c, h3, h4⟩,
+  { cases h3 },
+  { trivial },
+  { rw eq_of_mem_singleton h3 at h4,
+    exact h4 _ (or.inl rfl) },
+  { cases mem_append.elim_left h3 with h5 h5,
+    apply or.inl (ihp h1.left ⟨c, h5, h4⟩),
+    apply or.inr (ihq h1.right ⟨c, h5, h4⟩) },
+  { rcases mem_map.elim_left h3 with ⟨cc, h5, h6⟩,
+    cases cc with cl cr,
+    cases mem_product.elim_left h5 with hl hr,
+    rw ← h6 at h4,
+    cases forall_mem_append.elim_left h4 with hl' hr',
+    apply and.intro (ihp h1.left ⟨_, hl, _⟩) (ihq h1.right ⟨_, hr, _⟩);
+    assumption },
+  repeat {cases h1}
+end
 
-
-
-
-
+lemma fam_exv_of_dnf_fam_exv {p : form} :
+  quant_free p → (dnf p).fam_exv α → p.fam_exv α :=
+begin
+  intros h0 h1 M,
+  cases h1 M with v h1,
+  refine ⟨v, holds_of_dnf_holds p h0 h1⟩
+end
