src/tactic/nccc/skolemize.lean
@@ -1,8 +1,10 @@
 import .form
 
-local notation  `#` := term.var
-local notation  `&` := term.fnc
-local notation  t1 `^*` t2 := term.app t1 t2
+variable {α : Type}
+
+local notation  `⅋`     := atom.sym
+local notation  a `&` b := atom.app a b
+local notation  a `#` k := atom.vpp a k
 
 local notation  `⊤*` := form.true
 local notation  `⊥*` := form.false
@@ -11,6 +13,10 @@ local notation  p `∧*` q := form.and p q
 local notation  p `∨*` q := form.or p q
 local notation  `∀*` := form.fa
 local notation  `∃*` := form.ex
+
+def skolem_term : atom → list nat → atom
+| a []      := a
+| a (k::ks) := skolem_term (a # k) ks
 
 def skolemize_core : nat → form → (nat × form)
 | k ⊤*       := (k, ⊤*)
@@ -26,18 +32,76 @@ def skolemize_core : nat → form → (nat × form)
   (n, p' ∧* q')
 | k (∀* p) :=
   let (m, p') := skolemize_core k p in
-  let ts := (p'.free_vdxs 1).map (term.fnc ∘ nat.pred) in
-  (m + 1, p'.subst 0 (term.mk_app (& m) ts))
+  let ks := (free_vdxs p').filter (λ x, 0 < x) in
+  (m + 1, (p'.subst 0 (skolem_term (⅋ m) ks)).decr_vdxs)
 | k (∃* p) :=
   let (m, p') := skolemize_core k p in
   (m, ∃* p')
 
+#exit
 def skolemize (p : form) : form :=
-let k := fresh_sdx p in
+let k := p.fresh_sdx in
 let (_,p') := skolemize_core k p in
 p'
 
--- lemma valid_skolemize_core_imp (α : Type) (p : form) :
+lemma closed_skolemize_core_aux (ks ms : list nat) :
+  ks = [] → ms = [] → ks ∪ ms = [] :=
+by {intros h0 h1, rw [h0, h1], refl}
 
-lemma valid_skolemize_imp (α : Type) (p : form) :
-  (skolemize p).valid α → p.valid α := sorry
+open list
+
+lemma free_vdxs_skolemize_core_subset :
+  ∀ k : nat, ∀ p : form,
+  free_vdxs (skolemize_core k p).snd ⊆ free_vdxs p
+| k ⊤*  := subset.refl _
+| k ⊥*  := subset.refl _
+| k ⟪l⟫ := subset.refl _
+
+#exit
+| k (p ∨* q) :=
+  begin
+    unfold skolemize_core,
+    cases h1 : (skolemize_core k p) with m p',
+    unfold skolemize_core,
+    cases h2 : (skolemize_core m q) with n q',
+    have hp : free_vdxs p' = free_vdxs p,
+    { simpa only [h1] using free_vdxs_skolemize_core k p },
+    have hq : free_vdxs q' = free_vdxs q,
+    { simpa only [h2] using free_vdxs_skolemize_core m q },
+    apply fun_mono_2 hp hq
+  end
+| k (p ∧* q) :=
+  begin
+    unfold skolemize_core,
+    cases h1 : (skolemize_core k p) with m p',
+    unfold skolemize_core,
+    cases h2 : (skolemize_core m q) with n q',
+    have hp : free_vdxs p' = free_vdxs p,
+    { simpa only [h1] using free_vdxs_skolemize_core k p },
+    have hq : free_vdxs q' = free_vdxs q,
+    { simpa only [h2] using free_vdxs_skolemize_core m q },
+    apply fun_mono_2 hp hq
+  end
+| k (∀* p) :=
+  begin
+
+  end
+| k (∃* p) :=
+  begin
+    unfold skolemize_core,
+    cases h1 : (skolemize_core k p) with m p',
+    apply (congr_arg (λ x : list nat,
+      (x.filter ((<) 0)).map nat.pred) _),
+    simpa only [h1] using free_vdxs_skolemize_core k p
+  end
+
+
+#check free_vdxs
+
+
+lemma closed_skolemize {p : form} :
+  closed p → closed (skolemize p) := sorry
+
+
+lemma fam_fav_of_fam_fav_skolemize {p : form} :
+  (skolemize p).fam_fav α → p.fam_fav α := sorry
