src/tactic/nccc/misc.lean
@@ -1,4 +1,4 @@
-variables {α : Type}
+variables {α β γ : Type}
 
 def update (m : nat) (a : α) (v : nat → α) : nat → α
 | n := if n = m then a else v n
@@ -13,3 +13,15 @@ meta def list_reflect [has_reflect α] (l : list α) : list expr :=
 l.map (λ x, `(x).to_expr)
 
 local notation f `₀↦` a := update_zero a f
+
+lemma fun_mono_2 {p : α → β → γ} {a1 a2 : α} {b1 b2 : β} :
+  a1 = a2 → b1 = b2 → (p a1 b1 = p a2 b2) :=
+λ h1 h2, by rw [h1, h2]
+
+lemma pred_mono_2 {p : α → β → Prop} {a1 a2 : α} {b1 b2 : β} :
+  a1 = a2 → b1 = b2 → (p a1 b1 ↔ p a2 b2) :=
+λ h1 h2, by rw [h1, h2]
+
+lemma pred_mono_2' {c : Prop → Prop → Prop} {a1 a2 b1 b2 : Prop} :
+  (a1 ↔ a2) → (b1 ↔ b2) → (c a1 b1 ↔ c a2 b2) :=
+λ h1 h2, by rw [h1, h2]
