src/tactic/nccc/pnf.lean
@@ -1,5 +1,6 @@
 import .form
 
+variable {α : Type}
 
 local notation  `⊤*` := form.true
 local notation  `⊥*` := form.false
@@ -9,25 +10,16 @@ local notation  p `∨*` q := form.or p q
 local notation  `∀*` := form.fa
 local notation  `∃*` := form.ex
 
--- | ⊤*        := sorry
--- | ⊥*        := sorry
--- | ⟪⟨s, k, ts⟩⟫ := sorry
--- | (p ∧* q)  := sorry
--- | (p ∨* q)  := sorry
--- | (∀* p)  := sorry
--- | (∃* p)  := sorry
-
 def pnf_right (c : form → form → form) : form → form → form
-| p (∀* q) := ∀* (pnf_right (p.incr_vdx 0) q)
-| p (∃* q) := ∃* (pnf_right (p.incr_vdx 0) q)
+| p (∀* q) := ∀* (pnf_right (p.incr_vdxs 0) q)
+| p (∃* q) := ∃* (pnf_right (p.incr_vdxs 0) q)
 | p      q := c p q
 
 def pnf_left (c : form → form → form) : form → form → form
-| (∀* p) q := ∀* (pnf_left p (q.incr_vdx 0))
-| (∃* p) q := ∃* (pnf_left p (q.incr_vdx 0))
+| (∀* p) q := ∀* (pnf_left p (q.incr_vdxs 0))
+| (∃* p) q := ∃* (pnf_left p (q.incr_vdxs 0))
 | p      q := pnf_right c p q
 
-/- Assumes ∀-free input formulas -/
 def pnf : form → form
 | ⊤*       := ⊤*
 | ⊥*       := ⊥*
@@ -37,7 +29,5 @@ def pnf : form → form
 | (∀* p)   := ∀* (pnf p)
 | (∃* p)   := ∃* (pnf p)
 
--- lemma valid_skolemize_core_imp (α : Type) (p : form) :
-
-lemma valid_pnf_imp (α : Type) (p : form) :
-  (pnf p).valid α → p.valid α := sorry
+lemma fam_fav_of_fam_fav_pnf {p : form} :
+  (pnf p).fam_fav α → p.fam_fav α := sorry
