src/tactic/nccc/search.lean
@@ -3,24 +3,27 @@ import .misc .mat
 universes u v
 variables {α β : Type}
 
-local notation  `⅋`   := term.fnc
-local notation  t `&` s := term.tpp t s
-local notation  t `#` k := term.vpp t k
+local notation  `⅋`   := atom.sym
+local notation  t `&` s := atom.app t s
+local notation  t `#` k := atom.vpp t k
 
 meta def clax : Type := list expr
 meta def subx : Type := list (nat × expr)
 
-@[reducible] meta def search.goal : Type := clax × clax × mat
+meta def subx.eval : subx → tactic sub
+| []             := return []
+| ((k, x) :: σx) :=
+  do a ← tactic.eval_expr atom x,
+     σ ← subx.eval σx,
+     return ((k, a) :: σ)
 
-meta inductive search.rule : Type
---| rot_p : nat → search.rule
---| rot_c : nat → search.rule
---| rot_m : nat → search.rule
---| start : subx → search.rule
-| red   : nat → search.rule
-| ext   : nat → nat → subx → search.rule
+@[reducible] meta def sgoal : Type := clax × clax × mat
 
-meta def goal.to_format : search.goal → format
+meta inductive rule : Type
+| red : nat → rule
+| ext : nat → nat → subx → rule
+
+meta def sgoal.to_format : sgoal → format
 | (Px, Cx, M) :=
   "(" ++
   "Path : " ++ Px.to_format ++
@@ -28,13 +31,9 @@ meta def goal.to_format : search.goal → format
   ", Matrix : " ++ M.to_format ++
   ")"
 
-meta instance goal.has_to_format : has_to_format search.goal := ⟨goal.to_format⟩
+meta instance sgoal.has_to_format : has_to_format sgoal := ⟨sgoal.to_format⟩
 
 meta def rule.to_format : rule → format
---| (rule.rot_p k) := "Rot-P " ++ k.repr
---| (rule.rot_c k) := "Rot-C " ++ k.repr
---| (rule.rot_m k) := "Rot-M " ++ k.repr
---| (rule.start σ) := "Start " ++ " _"
 | (rule.red k)     := "Red " ++ k.repr
 | (rule.ext j i σ) := "Ext " ++ j.repr ++ " " ++ i.repr ++ " _"
 
@@ -43,14 +42,14 @@ meta instance rule.has_to_format : has_to_format rule := ⟨rule.to_format⟩
 meta structure search_state :=
 (max : nat)
 (lim : nat)
-(goals : list search.goal)
-(rules : list search.rule)
+(sgoals : list sgoal)
+(rules : list rule)
 
 meta def search_state.to_format : search_state → format
 | ⟨m, l, gs, rs⟩ :=
   "Max : " ++ m.repr ++ "\n" ++
   "Lim : " ++ l.repr ++ "\n" ++
-  "Goals : " ++ gs.to_format ++ "\n" ++
+  "S-Goals : " ++ gs.to_format ++ "\n" ++
   "Rules : " ++ rs.to_format ++ "\n"
 
 meta instance search_state.has_to_format : has_to_format search_state :=
@@ -70,24 +69,24 @@ namespace search
 
 meta def get_max : search nat := search_state.max <$> get
 meta def get_lim : search nat := search_state.lim <$> get
-meta def get_goals : search (list goal) := search_state.goals <$> get
+meta def get_sgoals : search (list sgoal) := search_state.sgoals <$> get
 meta def get_rules : search (list rule) := search_state.rules <$> get
 
 meta def set_max (m : nat) : search unit := modify $ λ s, {max := m, .. s}
 meta def set_lim (l : nat) : search unit := (modify $ λ s, {lim := l, .. s})
-meta def set_goals (gs : list goal) : search unit := modify $ λ s, {goals := gs, .. s}
+meta def set_goals (gs : list sgoal) : search unit := modify $ λ s, {sgoals := gs, .. s}
 meta def set_rules (rs : list rule) : search unit := modify $ λ s, {rules := rs, .. s}
 
-meta def pop_goal : search goal :=
-do (g::gs) ← get_goals,
+meta def pop_goal : search sgoal :=
+do (g::gs) ← get_sgoals,
    set_goals gs,
    return g
 
 meta def print [has_to_tactic_format α] (a : α) : search unit :=
 state_t.lift (tactic.trace a)
 
-meta def push_goal (g : goal) : search unit :=
-do gs ← get_goals,
+meta def push_goal (g : sgoal) : search unit :=
+do gs ← get_sgoals,
    set_goals (g::gs)
 
 meta def push_rule (r : rule) : search unit :=
@@ -111,6 +110,9 @@ b >>>= (λ _, s)
 
 infixr `>>>` : 1100 := bthen
 
+meta def trace {α : Type u} [has_to_tactic_format α] (a : α) : search unit :=
+state_t.lift (tactic.trace a)
+
 meta def pick_lim : search (backtrack unit) :=
 do m ← get_max,
    l ← get_lim,
@@ -120,41 +122,30 @@ meta def subx.mk : list nat → tactic subx
 | []      := return []
 | (k::ks) :=
   do sx ← subx.mk ks,
-     tx ← tactic.mk_meta_var `(term),
+     tx ← tactic.mk_meta_var `(atom),
      return ((k,tx)::sx)
 
-meta def termx.mk_aux (tx : expr) (k : nat) : subx → expr
+meta def atomx.mk_aux (tx : expr) (k : nat) : subx → expr
 | []          := `(%%tx # %%`(k))
 | ((m,sx)::σ) :=
-  if k = m then `(%%tx & %%sx) else termx.mk_aux σ
+  if k = m then `(%%tx & %%sx) else atomx.mk_aux σ
 
-meta def termx.mk (σ : subx) : term → expr
+meta def atomx.mk (σ : subx) : atom → expr
 | (⅋ k)   := `(⅋ k)
-| (t & s) := `(%%(termx.mk t) & %%(termx.mk s))
-| (t # k) := termx.mk_aux (termx.mk t) k σ
-
-meta def termsx.mk (σ : subx) : list term → expr
-| []      := `(@list.nil term)
-| (t::ts) := `(@list.cons term %%(termx.mk σ t) %%(termsx.mk ts))
+| (t & s) := `(%%(atomx.mk t) & %%(atomx.mk s))
+| (t # k) := atomx.mk_aux (atomx.mk t) k σ
 
 meta def litx.mk (σ : subx) : lit → expr
-| ⟨b, k, ts⟩ := `(lit.mk %%`(b) %%`(k) %%(termsx.mk σ ts))
+| ⟨b, a⟩ := `(@prod.mk bool atom %%`(b) %%(atomx.mk σ a))
 
 meta def pick_cla_aux (M : mat) (k : nat) : search unit :=
 match M.rotate k with
 | []        := failed
 | (C :: M') :=
   if cla.is_pos C
-  then --match cla.vdxs C with
-       --| []        :=
-       --  do push_goal ([], C.map (litx.mk []), M'),
-       --     push_rule (rule.rot_m k),
-       --     push_rule (rule.start [])
-       --| vs@(_::_) :=
-         do σ ← state_t.lift (subx.mk $ C.vdxs),
-            push_goal ([], C.map (litx.mk σ), if σ = [] then M' else M),
-            push_rule (rule.ext k 0 σ)
-       --end
+  then do σ ← state_t.lift (subx.mk $ C.vdxs),
+          push_goal ([], C.map (litx.mk σ), if σ = [] then M' else M),
+          push_rule (rule.ext k 0 σ)
   else failed
 end
 
@@ -163,8 +154,8 @@ do (_, _, M) ← pop_goal,
    return (pick_cla_aux M, M.length)
 
 meta def negx.mk : expr → search expr
-| `(lit.mk %%bx %%kx %% tsx) :=
-  return `(lit.mk (bnot %%bx) %%kx %% tsx)
+| `(@prod.mk bool atom %%bx %%ax) :=
+  return `(@prod.mk bool atom (bnot %%bx) %%ax)
 | _ := failed
 
 meta def comp_unify (L N : expr): search unit :=
@@ -213,7 +204,6 @@ meta def extend : bsearch unit :=
 ( ( do
   l ← get_lim,
   (Px, Lx::Cx, M) ← pop_goal,
-  state_t.lift (tactic.trace "Current matrix : " >> tactic.trace M),
   if Px.length < l
   then return (extend_aux Lx Px Cx M, M.length * maxlen M)
   else failed )
@@ -223,14 +213,14 @@ meta def close : search unit :=
 do ⟨_, [], _⟩ ← pop_goal, skip
 
 meta def finish : search unit :=
-do gs ← get_goals,
+do gs ← get_sgoals,
    if gs = [] then skip else failed
 
 local attribute [inline] state_t.orelse
 
 meta def loop : search unit :=
-(reduce >>> loop) <|> (extend >>> loop) <|>
-  (close >> loop) <|> finish
+((reduce >>> loop) <|> (extend >>> loop) <|>
+  (close >> loop) <|> finish)
 
 meta def main : search unit :=
 pick_lim >>> pick_cla >>> loop
@@ -239,13 +229,15 @@ meta def mk_search_state (M : mat) (l : nat := M.length)
   (m : nat := l * 2) : tactic search_state :=
 return ⟨m, l, [⟨[], [], M⟩], []⟩
 
-meta def derive (M : mat) : tactic (list rule) :=
-(list.reverse ∘ search_state.rules) <$> prod.snd <$>
-  (mk_search_state M >>= @state_t.run search_state tactic unit main)
-
 end search
 
+meta def derive (M : mat) : tactic (list rule) :=
+(list.reverse ∘ search_state.rules) <$> prod.snd <$>
+  (search.mk_search_state M >>= @state_t.run search_state tactic unit search.main)
+
 #exit
-def socrates : mat := [[⟨tt, 0, [⅋ 0]⟩, ⟨tt, 1, [⅋ 1]⟩], [⟨ff, 0, [⅋ 0]⟩], [⟨ff, 1, [⅋ 1]⟩]]
+def socrates : mat :=
+  [[⟨tt, (⅋ 0) & (⅋ 0)⟩,   ⟨tt, (⅋ 1) & (⅋ 1)⟩],
+   [⟨ff, (⅋ 0) & (⅋ 0)⟩], [⟨ff, (⅋ 1) & (⅋ 1)⟩]]
 
 run_cmd derive socrates >>= tactic.trace
