src/tactic/nccc/univ_close.lean
@@ -1,0 +1,46 @@
+import .form
+
+variable {α : Type}
+
+local notation  `⊤*` := form.true
+local notation  `⊥*` := form.false
+local notation  `⟪` l `⟫` := form.lit l
+local notation  p `∨*` q := form.or p q
+local notation  p `∧*` q := form.and p q
+local notation  `∀*` := form.fa
+local notation  `∃*` := form.ex
+
+local notation m `↦` a := update m a
+
+def univ_close_core (p : form) :
+  nat → model α → Prop
+| 0     M :=  p.holds M (λ _, M.inhab)
+| (k+1) M :=
+  match p.symb_arity k with
+  | none   := ∀ u : unit, univ_close_core k M
+  | some (tt,m) :=
+    ∀ r : arity α Prop m, univ_close_core k
+    {M with rels  := (k ↦ r.app_list _root_.false) M.rels}
+  | some (ff,m) :=
+    ∀ f : arity α α m, univ_close_core k
+    {M with funs := (k ↦ f.app_list M.inhab) M.funs}
+  end
+
+lemma univ_close_core_of_fam_fav (p : form) (h1 : p.fam_fav α) :
+  ∀ (k : nat) (M : model α), univ_close_core p k M
+| 0 M     := by apply h1
+| (k+1) M :=
+  begin
+    unfold univ_close_core,
+    cases (p.symb_arity k) with bm,
+    { intro _, apply univ_close_core_of_fam_fav },
+    { cases bm with b m, cases b;
+      intro _; apply univ_close_core_of_fam_fav }
+  end
+
+def univ_close (α : Type) [h : inhabited α] (p : form) : Prop :=
+univ_close_core p p.fresh_sdx (model.default α)
+
+lemma univ_close_of_fam_fav [h : inhabited α] {p : form} :
+  p.fam_fav α → univ_close α p :=
+λ h1, univ_close_core_of_fam_fav _ h1 _ _
